firmware/LibBase/BitfieldProperties.v
@@ -20,6 +20,7 @@ Require Import coqutil.Tactics.Tactics.
 Require Import coqutil.Tactics.syntactic_unify.
 Require Import coqutil.Tactics.letexists.
 Require Import coqutil.Z.Lia.
+Require Import Bedrock2Experiments.ProgramSemantics32.
 Require Import Bedrock2Experiments.Tactics.
 Require Import Bedrock2Experiments.WhileProperties.
 Require Import Bedrock2Experiments.Word.
@@ -32,11 +33,13 @@ Local Open Scope list_scope.
 Local Open Scope Z_scope.
 
 Section Proof.
-  Context {p : parameters} {p_ok : parameters_ok p}.
+  Context {word: word.word 32} {mem: map.map word Byte.byte}
+          {word_ok: word.ok word} {mem_ok: map.ok mem}
+          {ext_spec: ExtSpec} {ext_spec_ok: ext_spec.ok ext_spec}.
 
   Global Instance spec_of_bitfield_field32_read : spec_of "b2_bitfield_field32_read" :=
     fun function_env =>
-      forall (field mask index : Semantics.word) (m : mem) (t : trace),
+      forall (field mask index : word) (m : mem) (t : trace),
         call function_env bitfield_field32_read t m [field; mask; index]
           (fun t' m' rets =>
           t = t' /\ m = m' /\ rets = [select_bits field index mask]
@@ -52,7 +55,7 @@ Section Proof.
 
   Global Instance spec_of_bitfield_bit32_read : spec_of "b2_bitfield_bit32_read" :=
     fun function_env =>
-      forall (field : Semantics.word) (index: Semantics.word) (m : mem) (t : trace),
+      forall (field : word) (index: word) (m : mem) (t : trace),
         call function_env bitfield_bit32_read t m [field; index]
           (fun t' m' rets =>
           t = t' /\ m = m' /\
@@ -63,20 +66,10 @@ Section Proof.
     program_logic_goal_for_function! bitfield_bit32_read.
   Proof.
     repeat straightline.
-    eexists; ssplit; repeat straightline.
-    {
-      (* TODO: here we can't proceed with straightline so use straightline_with_map_lookup.
-         make it a bit verbose so that we can see where it's needed explicitly. *)
-      straightline_with_map_lookup.
-      repeat straightline.
-      straightline_with_map_lookup.
-      repeat straightline.
-    }
     (* call bitfield_field32_read *)
     straightline_call; eauto; try reflexivity; [ ].
-
-    repeat straightline_with_map_lookup.
+    unfold select_bits in *.
+    repeat straightline.
     repeat split; try reflexivity.
   Qed.
-
 End Proof.
