firmware/StateMachineMMIOSpec.v
@@ -7,42 +7,43 @@ Require Import coqutil.Map.Interface coqutil.Word.Interface.
 Require Import riscv.Utility.Utility.
 Require Import Bedrock2Experiments.Riscv.MinimalMMIO.
 Require Import Bedrock2Experiments.Riscv.MetricMinimalMMIO.
+Require Import Bedrock2Experiments.ProgramSemantics32.
 Require Import Bedrock2Experiments.StateMachineSemantics.
 
-Instance StateMachineMMIOSpec{W: Words}{mem: map.map word byte}
-         {parameters: StateMachineSemantics.parameters width word mem}: MMIOSpec :=
-  {| isMMIOAddr := parameters.isMMIOAddr;
+Instance StateMachineMMIOSpec{word: word.word 32}{mem: map.map word Byte.byte}
+         {M: state_machine.parameters}: MMIOSpec :=
+  {  isMMIOAddr := state_machine.isMMIOAddr;
      isMMIOAligned n a := word.unsigned a mod (Z.of_nat n) = 0;
      MMIOReadOK :=
        fun sz log addr val =>
          exists s s' r,
            execution log s
-           /\ parameters.reg_addr r = addr
-           /\ parameters.read_step sz s r val s';
+           /\ state_machine.reg_addr r = addr
+           /\ state_machine.read_step sz s r val s';
      MMIOWriteOK :=
        fun sz log addr val =>
          exists s s' r,
            execution log s
-           /\ parameters.reg_addr r = addr
-           /\ parameters.write_step sz s r val s';
-  |}.
+           /\ state_machine.reg_addr r = addr
+           /\ state_machine.write_step sz s r val s';
+  }.
 
 Section TODO_Why_not_like_this. (* (would also require a corresponding update in ext_spec) *)
-  Instance StateMachineMMIOSpec_Alt{W: Words}{mem: map.map word byte}
-           {parameters: StateMachineSemantics.parameters width word mem}: MMIOSpec :=
-    {| isMMIOAddr := parameters.isMMIOAddr;
+  Instance StateMachineMMIOSpec_Alt{word: word.word 32}{mem: map.map word Byte.byte}
+           {M: state_machine.parameters}: MMIOSpec :=
+    {| isMMIOAddr := state_machine.isMMIOAddr;
        isMMIOAligned n a := word.unsigned a mod (Z.of_nat n) = 0;
        MMIOReadOK :=
          fun sz log addr val =>
-           exists r, parameters.reg_addr r = addr /\
+           exists r, state_machine.reg_addr r = addr /\
                      (* for all states s that could be the explanation of the trace t,
                         this read_step must be possible *)
-                     forall s, execution log s -> exists s', parameters.read_step sz s r val s';
+                     forall s, execution log s -> exists s', state_machine.read_step sz s r val s';
        MMIOWriteOK :=
          fun sz log addr val =>
-           exists r, parameters.reg_addr r = addr /\
+           exists r, state_machine.reg_addr r = addr /\
                      (* for all states s that could be the explanation of the trace t,
                         this write_step must be possible *)
-                     forall s, execution log s -> exists s', parameters.write_step sz s r val s';
+                     forall s, execution log s -> exists s', state_machine.write_step sz s r val s';
     |}.
 End TODO_Why_not_like_this.
